LeanPy/Data/Dict/Object.lean
@@ -1,0 +1,116 @@
+/-
+Copyright (c) 2025 Mac Malone. All rights reserved.
+Released under the Apache 2.0 license as described in the file LICENSE.
+Authors: Mac Malone
+-/
+import LeanPy.Data.Dict.Ref
+import LeanPy.Data.Object.Slots
+import LeanPy.Data.Str.Object
+
+namespace LeanPy
+
+/- An instance of a subclass of `dict` that satisfies `p`. -/
+abbrev PDictObject (p : ObjectProp) := PSubObject p dictTypeRef
+
+/- An instance of a subclass of `dict`. -/
+def DictObject := PDictObject .Any
+
+/-- Returns whether this object is an instance of a subtype of `dict`. -/
+@[inline] def Object.isDict (self : Object) : Bool :=
+ self.ty.isDictSubclass
+
+/-- Casts `self` to `DictObject`. -/
+@[inline] def Object.asDict (self : Object) (h : self.isDict) : DictObject :=
+  self.asSubObject (self.ty.isDictSubclass_iff_subset.mp h)
+
+/--
+Casts `self` to `DictObject` if `self` is instance of a subtype of `dict`.
+Otherwise, returns `none`.
+-/
+@[inline] def Object.asDict? (self : Object) : Option DictObject :=
+  if h : self.isDict then some (self.asDict h) else none
+
+namespace ObjectData
+
+@[inline] private unsafe def ofDictRefImpl (dict : DictRef) : ObjectData :=
+  unsafeCast dict
+
+@[implemented_by ofDictRefImpl]
+abbrev ofDictRef (dict : DictRef) : ObjectData := .mkCore dictDataKind dict
+
+opaque getDictRef (self : ObjectData) (h : self.kind = dictDataKind) : DictRef :=
+  unsafe unsafeCast self
+
+end ObjectData
+
+namespace DictObject
+
+instance : Coe DictObject Object := ⟨PObject.toObject⟩
+
+theorem isDict_toObject (self : DictObject) : self.toObject.isDict :=
+  self.ty.isDictSubclass_iff_subset.mpr self.ty_subset
+
+@[inline] def getDictRef (self : DictObject) : DictRef :=
+  self.data.getDictRef (self.lawful_subobject).2
+
+/--
+Returns `true` if the two dictionaries are equal.
+
+This is equivalent to the Python `dict.__eq__(self, other)`.
+-/
+@[inline] protected def beqM (self other : DictObject) : PyM Bool :=
+  self.getDictRef.beqM other.getDictRef
+
+/--
+Returns `true` if the two dictionaries are not equal.
+
+This is equivalent to the Python `dict.__ne__(self, other)`.
+-/
+@[inline] protected def bneM (self other : DictObject) : PyM Bool :=
+  not <$> self.beqM other
+
+/--
+Return the number of items in the dictionary.
+
+This is equivalent to the Python `dict.len(self)`.
+-/
+@[inline] def lengthM (self : DictObject) : BaseIO Nat :=
+  (·.size) <$> self.getDictRef.get
+
+/-- Return `true` unless the dictionary is empty. -/
+@[inline] def toBoolM (self : DictObject) : BaseIO Bool :=
+  (· != 0) <$> self.lengthM
+
+/--
+Return a string representation of the dictionary.
+
+This is equivalent to the Python `dict.__repr__(self)`.
+-/
+@[inline] def reprM (self : DictObject) : PyM String :=
+  self.getDictRef.reprM
+
+end DictObject
+
+def throwUnhashableType (tyName : String) : PyM α := do
+  -- TODO: make this a TypeError
+  throw ((← mkStrObject s!"unhashable type: '{tyName}'") : ErrorObject)
+
+def dictTypeRef.slots : TObjectSlots DictObject where
+  hash _ := throwUnhashableType "dict"
+  beq self other :=
+    if let some other := other.asDict? then self.beqM other else return false
+  bne self other :=
+    if let some other := other.asDict? then self.beqM other else return true
+  bool self := self.toBoolM
+  repr self := self.reprM
+
+@[instance] initialize dictTypeSlotsRef : TypeSlots dictTypeRef ←
+  dictTypeRef.slots.mkRef
+
+@[inline] def DictObject.ofDictRef (r : DictRef) : DictObject :=
+  dictTypeRef.mkObjectCore r.id  (.ofDictRef r)
+
+instance : Coe DictRef DictObject := ⟨DictObject.ofDictRef⟩
+
+@[inline] def mkDictObject (data : DictRef.Data) : BaseIO DictObject :=
+  .ofDictRef <$> mkDictRef data
