LeanPy/Data/Dict/Ref.lean
@@ -1,0 +1,78 @@
+/-
+Copyright (c) 2025 Mac Malone. All rights reserved.
+Released under the Apache 2.0 license as described in the file LICENSE.
+Authors: Mac Malone
+-/
+import LeanPy.Data.HashDict
+import LeanPy.Data.None.Object
+import LeanPy.Data.Object.Slots
+
+namespace LeanPy
+
+@[inline] def mkDictRef (data : DictRef.Data) : BaseIO DictRef :=
+  mkMutableRef data
+
+namespace DictRef
+
+namespace Data
+
+def set (k : Object) (v : Object) (self : Data) : PyM Data := do
+  let hash ← k.hashM
+  let cell ← mkMutableRef v
+  let self ← self.raw.insertCoreM hash k cell (.up <$> k.beqM ·)
+  return ⟨self⟩
+
+end Data
+
+/--
+Returns `true` if the two dictionaries are equal.
+
+Dictionaries compare equal if and only if they have the same
+`(key, value)` pairs (regardless of ordering).
+-/
+-- Should follow the logic in CPython's `dict_equal`
+-- https://github.com/python/cpython/blob/3.11/Objects/dictobject.c#L3155
+def beqM (a b : DictRef) : PyM Bool := do
+  let a ← a.get
+  let b ← b.get
+  unless a.size == b.size do
+    return false
+  for entry in a.entries do
+    let .some ah ak av := entry
+      | continue
+    let ⟨bi⟩ ← b.raw.getEntryIdxCoreM ah (.up <$> ak.beqM ·)
+    let some (.some _ _ bv) := b.entries[bi]?
+      | return false
+    let av ← av.get
+    let bv ← bv.get
+    unless (← av.beqM bv) do
+      return false
+  return true
+
+/-- Returns a string representation of the dictionary. -/
+-- Should follow the logic in CPython's `dict_repr`
+-- https://github.com/python/cpython/blob/3.11/Objects/dictobject.c#L2403
+def reprM (self : DictRef) : PyM String := do
+  let es ← self.getAndMap (·.entries)
+  return (← appendHead "{" 0 es).push '}'
+where
+  appendHead s i entries : PyM String := do
+    if h : i < entries.size then
+      if let .some _ k v := entries[i] then
+        appendTail (← append s k v) (i+1) entries
+      else appendHead s (i+1) entries
+    else return s
+  termination_by entries.size - i
+  decreasing_by omega
+  appendTail s i entries := do
+    if h : i < entries.size then
+      if let .some _ k v := entries[i] then
+        appendTail (← append s!"{s}, " k v) (i+1) entries
+      else appendTail s (i+1) entries
+    else return s
+  termination_by entries.size - i
+  decreasing_by all_goals omega
+  append s k v := do
+    let k ← k.reprM
+    let v ← (← v.get).reprM
+    return s!"{s}{k}: {v}"
